src/program_proof/rsm/distx/program/txn.v
@@ -1,17 +1,28 @@
 From Perennial.program_proof.rsm.distx Require Import prelude.
 From Perennial.program_proof.rsm.distx.program Require Import replica_group.
+From Perennial.program_proof.rsm.distx.invariance Require Import linearize.
 From Goose.github_com.mit_pdos.rsm Require Import distx.
 
 Section program.
   Context `{!heapGS Σ, !distx_ghostG Σ}.
 
-  Definition txn_ptsto (τ : gname) (k : dbkey) (v : dbval) : iProp Σ.
+  Definition txnmap_auth (τ : gname) (m : dbmap) : iProp Σ.
   Admitted.
 
-  Definition txn_ptstos (τ : gname) (m : dbmap) : iProp Σ :=
-    [∗ map] k ↦ v ∈ m, txn_ptsto τ k v.
+  Definition txnmap_ptsto (τ : gname) (k : dbkey) (v : dbval) : iProp Σ.
+  Admitted.
+
+  Definition txnmap_ptstos (τ : gname) (m : dbmap) : iProp Σ :=
+    [∗ map] k ↦ v ∈ m, txnmap_ptsto τ k v.
+
+  Lemma txnmap_alloc m :
+    ⊢ |==> ∃ τ, txnmap_auth τ m ∗ ([∗ map] k ↦ v ∈ m, txnmap_ptsto τ k v).
+  Admitted.
 
   Definition own_txn_uninit (txn : loc) (γ : distx_names) : iProp Σ.
+  Admitted.
+
+  Definition own_txn_init (txn : loc) (tid : nat) (γ : distx_names) : iProp Σ.
   Admitted.
 
   (* TODO: we didn't expose [view] as in vMVCC, is that an issue? *)
@@ -33,9 +44,9 @@ Section program.
   Admitted.
 
   Theorem wp_Txn__Read (txn : loc) (tid : nat) (key : string) (value : dbval) γ τ :
-    {{{ own_txn txn tid γ τ ∗ txn_ptsto τ key value }}}
+    {{{ own_txn txn tid γ τ ∗ txnmap_ptsto τ key value }}}
       Txn__Read #txn #(LitString key)
-    {{{ RET (dbval_to_val value); own_txn txn tid γ τ ∗ txn_ptsto τ key value }}}.
+    {{{ RET (dbval_to_val value); own_txn txn tid γ τ ∗ txnmap_ptsto τ key value }}}.
   Proof.
     (*@ func (txn *Txn) Read(key string) Value {                                @*)
     (*@     gid := KeyToGroup(key)                                              @*)
@@ -53,9 +64,9 @@ Section program.
   Admitted.
 
   Theorem wp_Txn__Write (txn : loc) (tid : nat) (key : string) (value : string) γ τ :
-    {{{ own_txn txn tid γ τ ∗ (∃ vprev, txn_ptsto τ key vprev) }}}
+    {{{ own_txn txn tid γ τ ∗ (∃ vprev, txnmap_ptsto τ key vprev) }}}
       Txn__Write #txn #(LitString key) #(LitString value)
-    {{{ RET #(); own_txn txn tid γ τ ∗ txn_ptsto τ key (Some value) }}}.
+    {{{ RET #(); own_txn txn tid γ τ ∗ txnmap_ptsto τ key (Some value) }}}.
   Proof.
     (*@ func (txn *Txn) Write(key string, value string) {                       @*)
     (*@     gid := KeyToGroup(key)                                              @*)
@@ -69,9 +80,9 @@ Section program.
   Admitted.
 
   Theorem wp_Txn__Delete (txn : loc) (tid : nat) (key : string) (value : dbval) γ τ :
-    {{{ own_txn txn tid γ τ ∗ txn_ptsto τ key value }}}
+    {{{ own_txn txn tid γ τ ∗ txnmap_ptsto τ key value }}}
       Txn__Delete #txn #(LitString key)
-    {{{ RET #(); own_txn txn tid γ τ ∗ txn_ptsto τ key None }}}.
+    {{{ RET #(); own_txn txn tid γ τ ∗ txnmap_ptsto τ key None }}}.
   Proof.
     (*@ func (txn *Txn) Delete(key string) {                                    @*)
     (*@     gid := KeyToGroup(key)                                              @*)
@@ -121,12 +132,12 @@ Section program.
     (*@ }                                                                       @*)
   Admitted.
 
-  Theorem wp_Txn__begin (txn : loc) (γ : distx_names) :
+  Theorem wp_Txn__begin (txn : loc) γ :
     ⊢ {{{ own_txn_uninit txn γ }}}
       <<< ∀∀ (ts : nat), ts_auth γ ts >>>
-        Txn__begin #txn @ ↑distxN
+        Txn__begin #txn @ ↑tsNS
       <<< ∃∃ (ts' : nat), ts_auth γ ts' ∗ ⌜(ts < ts')%nat⌝ >>>
-      {{{ RET #(); ∃ τ, own_txn txn ts' γ τ }}}.
+      {{{ RET #(); own_txn_init txn ts' γ }}}.
   Proof.
     (*@ func (txn *Txn) begin() {                                               @*)
     (*@     // TODO                                                             @*)
@@ -195,11 +206,11 @@ Section program.
     (Rc : dbmap -> dbmap -> iProp Σ) (Ra : dbmap -> iProp Σ)
     γ τ : iProp Σ :=
     ∀ Φ,
-    own_txn txn tid γ τ ∗ ⌜P r⌝ ∗ txn_ptstos τ r -∗
+    own_txn txn tid γ τ ∗ ⌜P r⌝ ∗ txnmap_ptstos τ r -∗
     (∀ ok : bool,
        (own_txn txn tid γ τ ∗
         if ok
-        then ∃ w, ⌜Q r w ∧ dom w ⊆ dom r⌝ ∗ (Rc r w ∧ Ra r) ∗ txn_ptstos τ w
+        then ∃ w, ⌜Q r w ∧ dom w ⊆ dom r⌝ ∗ (Rc r w ∧ Ra r) ∗ txnmap_ptstos τ w
         else Ra r) -∗ Φ #ok) -∗
     WP body #txn {{ v, Φ v }}.
 
@@ -208,14 +219,35 @@ Section program.
     (P : dbmap -> Prop) (Q : dbmap -> dbmap -> Prop)
     (Rc : dbmap -> dbmap -> iProp Σ) (Ra : dbmap -> iProp Σ) γ :
     (∀ r w, (Decision (Q r w))) ->
-    ⊢ {{{ own_txn_uninit txn γ ∗ (∀ tid r τ, spec_body body txn tid r P Q Rc Ra γ τ) }}}
-      <<< ∀∀ (r : dbmap), ⌜P r⌝ ∗ db_ptstos γ r >>>
-        Txn__Run #txn body @ ↑distxN
-      <<< ∃∃ (ok : bool) (w : dbmap), if ok then ⌜Q r w⌝ ∗ db_ptstos γ (w ∪ r) else db_ptstos γ r >>>
-      {{{ RET #ok; own_txn_uninit txn γ ∗ if ok then Rc r w else Ra r }}}.
+    know_distx_inv γ -∗
+    {{{ own_txn_uninit txn γ ∗ (∀ tid r τ, spec_body body txn tid r P Q Rc Ra γ τ) }}}
+    <<< ∀∀ (r : dbmap), ⌜P r⌝ ∗ db_ptstos γ r >>>
+      Txn__Run #txn body @ ↑sysNS
+    <<< ∃∃ (ok : bool) (w : dbmap), if ok then ⌜Q r w⌝ ∗ db_ptstos γ (w ∪ r) else db_ptstos γ r >>>
+    {{{ RET #ok; own_txn_uninit txn γ ∗ if ok then Rc r w else Ra r }}}.
   Proof.
+    iIntros (Hdec) "#Hinv !>".
+    iIntros (Φ) "[Htxn Hbody] HAU".
+    wp_rec. wp_pures.
+
     (*@ func (txn *Txn) Run(body func(txn *Txn) bool) bool {                    @*)
     (*@     txn.begin()                                                         @*)
+    (*@                                                                         @*)
+    wp_apply (wp_Txn__begin with "Htxn").
+    iInv "Hinv" as "> HinvO" "HinvC".
+    iMod (ncfupd_mask_subseteq (⊤ ∖ ↑sysNS)) as "Hclose"; first solve_ndisj.
+    iMod "HAU" as (r) "[[%HP Hdbpts] HAUC]".
+    iModIntro.
+    iNamed "HinvO".
+    iDestruct (txnsys_inv_expose_future_extract_ts with "Htxn") as (future ts) "[Htxn Hts]".
+    (* Prove [key_inv] are linearizable after [ts]. *)
+    iDestruct (keys_inv_before_linearize with "Hkeys Hts") as "[Hkeys Hts]".
+    iExists ts.
+    (* Pass [ts_auth γ ts] to the underlying layer. *)
+    iFrame "Hts".
+    iIntros (tid) "[Hts %Htidgt]".
+    iDestruct (ts_witness with "Hts") as "#Htidlb".
+
     (*@     cmt := body(txn)                                                    @*)
     (*@     if !cmt {                                                           @*)
     (*@         // This transaction has not really requested to prepare yet, so no @*)
@@ -241,6 +273,35 @@ Section program.
     (*@     txn.commit()                                                        @*)
     (*@     return true                                                         @*)
     (*@ }                                                                       @*)
+    pose proof (peek_spec future tid) as Hpeek.
+    destruct (peek future tid).
+    { (* Case: No commit of timestamp [ts] in the future. *)
+      iMod (txnsys_inv_linearize_abort NC Q with "Htidlb Hdbpts Htxn Hkeys")
+        as "(Hdbpts & Htxn & Hkeys & Hwrsexcl & #HQ & #Hlnrzs & #Hlnrzed)".
+      { (* TODO: Prove [dom r ⊆ keys_all]. *) admit. }
+      { apply Htidgt. }
+      { apply Hpeek. }
+      { done. }
+      (* Choose the will-abort branch. Use [∅] as placeholder. *)
+      iMod ("HAUC" $! false ∅ with "Hdbpts") as "HΦ".
+      iMod "Hclose" as "_".
+      iMod ("HinvC" with "[Htxn Hkeys Hgroups]") as "_".
+      { admit. }
+      (* Allocate transaction local view [txnmap_ptstos τ r]. *)
+      iMod (txnmap_alloc r) as (τ) "[Htxnmap Htxnpts]".
+      iIntros "!> Htxn".
+      iAssert (own_txn txn tid γ τ)%I with "[Htxn Htxnmap]" as "Htxn".
+      { admit. }
+      wp_apply ("Hbody" with "[$Htxn $Htxnpts]"); first done.
+      iIntros (cmt) "[Htxn Hpost]".
+      wp_pures.
+      wp_if_destruct.
+      { iApply "HΦ".
+        (* TODO: weaken [own_txn] to [own_txn_uninit]. *)
+        admit.
+      }
+      wp_apply (wp_Txn__prepare with "Htxn").
+      iIntros (status) "[Htxn Hstatus]".
   Admitted.
 
 End program.
