src/program_proof/rsm/vos.sh
@@ -2,7 +2,7 @@
 
 dir='./src/program_proof/rsm'
 
-cd ../../../
+cd "$(dirname $0)"/../../../
 files=`find ${dir} -name "${1}*.v" ! -name "print_assumptions.v" | sed "s/\.v/\.vos/"`
 if [[ -z ${files} ]]; then
     echo "No target files."
